update

ironfleet/src/Dafny/Distributed/LockProof/proof.i.dfy
@@ -1,16 +1,14 @@
 include "../Protocol/Lock/RefinementProof/DistributedSystem.i.dfy"
 include "../Protocol/Lock/Node.i.dfy"
 include "../Services/Lock/AbstractService.s.dfy"
+include "p_s_correspondence.s.dfy"
+
 
 module LockProof {
 import opened DistributedSystem_i
 import opened Protocol_Node_i
 import opened AbstractServiceLock_s
-
-
-lemma sameServers(s:LS_State, s':LS_State)
-requires LS_Next(s, s')
-ensures forall e :: e in s.servers <==> e in s'.servers
+import opened P_S_Correspondence_s
 
 lemma sameConfig(config:Config, ls:seq<LS_State>)
 requires |ls| > 0
@@ -46,6 +44,8 @@ ensures forall i :: 0 <= i < |gls|-1 ==> GLS_Next(gls[i], gls[i+1]) || gls[i] ==
 ensures forall i :: 0 <= i < |gls|-1 ==> (gls[i].history == gls[i+1].history || exists new_holder :: new_holder in config && gls[i+1].history == gls[i].history + [new_holder])
 ensures gls[|gls|-1].ls == ls[|ls|-1]
 ensures forall i :: 0 <= i < |ls| ==> gls[i].ls == ls[i]
+ensures forall i :: 0 <= i < |ls|-1 ==> (ls[i] == ls[i+1] ==> gls[i] == gls[i+1])
+ensures forall i :: 0 <= i < |ls| ==> LS_GLS_Correspondence(ls[i].environment.sentPackets, gls[i], config)
 {
     if (|ls| == 1) {
         gls := [GLS_State(ls[0], [config[0]])];
@@ -56,7 +56,6 @@ ensures forall i :: 0 <= i < |ls| ==> gls[i].ls == ls[i]
         assert(|gls| == |ls|-1);
         var history := gls[|gls|-1].history;
 
-        assert forall i :: 0 <= i < |ls|-1 ==> (LS_Next(ls[i], ls[i+1]) || ls[i] == ls[i+1]);
         assert forall i :: 0 <= i < |ls|-1 ==> (!LS_Next(ls[i], ls[i+1]) ==> ls[i] == ls[i+1]);
         var xxx := |ls|-2;
         assert(0 <= xxx < |ls|-1);
@@ -76,23 +75,7 @@ ensures forall i :: 0 <= i < |ls| ==> gls[i].ls == ls[i]
                 assert LS_Init(ls[0], config);
                 assert forall i :: 0 <= i < |ls|-1 ==> LS_Next(ls[i], ls[i+1]) || ls[i] == ls[i+1];
 
-
-                assert forall j :: j in ls[0].servers ==> ls[0].servers[j].config == config;
-                
-                var k := 1;
-                while (k < |ls|) 
-                invariant 1 <= k <= |ls|
-                invariant forall i :: 0 <= i < k ==> forall j :: j in ls[i].servers ==> ls[i].servers[j].config == config;
-                {
-                    assert forall i :: 0 <= i < k ==> forall j :: j in ls[i].servers ==> ls[i].servers[j].config == config;
-                    assert 0 <= k-1 < |ls|-1;
-                    assert (ls[k-1] == ls[k] || LS_Next(ls[k-1], ls[k]));
-                    assert forall j :: j in ls[k].servers ==> ls[k].servers[j].config == ls[k-1].servers[j].config;
-                    assert forall i :: 0 <= i <= k ==> forall j :: j in ls[i].servers ==> ls[i].servers[j].config == config;
-                    k := k + 1;
-                }
-                // I have a lemma for this large chunk of proof. But Dafny does not use it!
-
+                sameConfig(config, ls);
 
                 assert forall i :: 0 <= i < |ls| ==> forall j :: j in ls[i].servers ==> ls[i].servers[j].config == config;
 
@@ -100,10 +83,42 @@ ensures forall i :: 0 <= i < |ls| ==> gls[i].ls == ls[i]
                 assert ls[|ls|-2].servers[ls[|ls|-2].environment.nextStep.actor].config == config;
                 assert ls[|ls|-2].servers[ls[|ls|-2].environment.nextStep.actor].config[(ls[|ls|-2].servers[ls[|ls|-2].environment.nextStep.actor].my_index + 1) % |ls[|ls|-2].servers[ls[|ls|-2].environment.nextStep.actor].config|] in config;
 
-                history := history + [ls[|ls|-2].servers[ls[|ls|-2].environment.nextStep.actor].config[(ls[|ls|-2].servers[ls[|ls|-2].environment.nextStep.actor].my_index + 1) % |ls[|ls|-2].servers[ls[|ls|-2].environment.nextStep.actor].config|]];
-                gls := gls + [GLS_State(ls[|ls|-1], history)];
-            } else 
-            {
+//                 history := history + [ls[|ls|-2].servers[ls[|ls|-2].environment.nextStep.actor].config[(ls[|ls|-2].servers[ls[|ls|-2].environment.nextStep.actor].my_index + 1) % |ls[|ls|-2].servers[ls[|ls|-2].environment.nextStep.actor].config|]];
+//                 gls := gls + [GLS_State(ls[|ls|-1], history)];
+
+                var s := ls[|ls|-2];
+                var s' := ls[|ls|-1];
+                var id := s.environment.nextStep.actor;
+                var ios := s.environment.nextStep.ios;
+                var packets := s.environment.sentPackets;
+                var packets' := s'.environment.sentPackets;
+
+                history := history + [s.servers[id].config[(s.servers[id].my_index + 1) % |s.servers[id].config|]];
+                gls := gls + [GLS_State(s', history)];
+
+                if (NodeGrant(s.servers[id], s'.servers[id], ios)) {
+                    if (s.servers[id].held && s.servers[id].epoch < 0xFFFF_FFFF_FFFF_FFFF) {
+                        assert |ios| == 1;
+                        assert ios[0].LIoOpSend?;
+                        assert ios[0].s.msg.Transfer?;
+                        assert forall p ::
+                                      p in packets
+                                   && p.src in s.servers
+                                   && p.dst in s.servers
+                                   && p.msg.Locked?
+                                 <==> p in packets'
+                                  && p.src in s'.servers
+                                  && p.dst in s'.servers
+                                  && p.msg.Locked?;
+                    } else {
+                    }
+                }
+
+
+
+
+            } else {
+
                 gls := gls + [GLS_State(ls[|ls|-1], history)];
             }
         } else 
@@ -118,27 +133,101 @@ ensures forall i :: 0 <= i < |ls| ==> gls[i].ls == ls[i]
             assert(gls[|gls|-1] == gls[|gls|-2] || GLS_Next(gls[|gls|-2], gls[|gls|-1]));
         }
 
-        //assert(forall i :: i in ls ==> forall j :: j in i.servers ==> i.servers[j].config == config);
-        //assert(forall i :: i in ls[|ls|-2].servers ==> ls[|ls|-2].servers[i].config == config);
+        assert LS_GLS_Correspondence(ls[|ls|-1].environment.sentPackets, gls[|gls|-1], config);
 
-        // if (ls[|ls|-2].environment.nextStep.LEnvStepHostIos? 
-        //         && ls[|ls|-2].environment.nextStep.actor in ls[|ls|-2].servers
-        //         && NodeGrant(ls[|ls|-2].servers[ls[|ls|-2].environment.nextStep.actor], ls[|ls|-1].servers[ls[|ls|-2].environment.nextStep.actor], ls[|ls|-2].environment.nextStep.ios)
-        //         && ls[|ls|-2].servers[ls[|ls|-2].environment.nextStep.actor].held 
-        //         && ls[|ls|-2].servers[ls[|ls|-2].environment.nextStep.actor].epoch < 0xFFFF_FFFF_FFFF_FFFF) {
-        //         assert(false);
-        //     history := history + [ls[|ls|-2].servers[ls[|ls|-2].environment.nextStep.actor].config[(ls[|ls|-2].servers[ls[|ls|-2].environment.nextStep.actor].my_index + 1) % |ls[|ls|-2].servers[ls[|ls|-2].environment.nextStep.actor].config|]];
-        //     gls := gls + [GLS_State(ls[|ls|-1], history)];
-        //     assert(GLS_Next(gls[|gls|-2], gls[|gls|-1]));
-        // } else {
-        //     gls := gls + [GLS_State(ls[|ls|-1], history)];
-        // }
-
-            
-
-        //assert(gls[|gls|-1] == gls[|gls|-2] || GLS_Next(gls[|gls|-2], gls[|gls|-1]));
     }
 }
+
+
+predicate LS_GLS_Correspondence(packets:set<LockPacket>, gls:GLS_State, config:Config) {
+    
+    forall p ::
+           p in packets
+        && p.src in config
+        && p.dst in config
+        && p.msg.Locked?
+        ==> var epoch := p.msg.locked_epoch;
+                0 < epoch <= |gls.history|
+            && p.src == gls.history[epoch-1]
+}
+
+
+// lemma LSToGLS_extended(config:Config, ls:seq<LS_State>) returns (gls:seq<GLS_State>)
+// requires |ls| > 0
+// requires LS_Init(ls[0], config)
+// requires forall i :: 0 <= i < |ls|-1 ==> LS_Next(ls[i], ls[i+1]) || ls[i] == ls[i+1]
+// ensures |ls| == |gls|
+// ensures GLS_Init(gls[0], config)
+// ensures forall i :: 0 <= i < |gls|-1 ==> GLS_Next(gls[i], gls[i+1]) || gls[i] == gls[i+1]
+// ensures forall i :: 0 <= i < |gls|-1 ==> (gls[i].history == gls[i+1].history || exists new_holder :: new_holder in config && gls[i+1].history == gls[i].history + [new_holder])
+// ensures gls[|gls|-1].ls == ls[|ls|-1]
+// ensures forall i :: 0 <= i < |ls| ==> gls[i].ls == ls[i]
+// ensures forall i :: 0 <= i < |ls|-1 ==> (ls[i] == ls[i+1] ==> gls[i] == gls[i+1])
+// ensures forall i :: 0 <= i < |ls| ==> LS_GLS_Correspondence(ls[i].environment.sentPackets, gls[i])
+// {
+//     gls := LSToGLS(config, ls);
+//     
+//     assert LS_GLS_Correspondence(ls[0].environment.sentPackets, gls[0]);
+//     var k := 1;
+//     while (k < |ls|)
+//     invariant 1 <= k <= |ls|
+//     invariant forall i :: 0 <= i < k ==> LS_GLS_Correspondence(ls[i].environment.sentPackets, gls[i]);
+//     {
+//         if (ls[k-1] == ls[k]) {
+//             var kk := k-1;
+//             assert gls[kk] == gls[kk+1];
+//             assert LS_GLS_Correspondence(ls[k].environment.sentPackets, gls[k]);
+//         } else {
+//             var packets := ls[k-1].environment.sentPackets;
+//             var packets' := ls[k].environment.sentPackets;
+//             if (ls[k-1].environment.nextStep.LEnvStepHostIos?
+//              && ls[k-1].environment.nextStep.actor in ls[k-1].servers) {
+// 
+//              // must be the case that LS_NextOneServer(ls[k-1], ls[k], ls[k-1].environment.nextStep.actor, ls[k-1].environment.nextStep.ios)
+//                 var s := ls[k-1];
+//                 var s' := ls[k];
+//                 var id := s.environment.nextStep.actor;
+//                 var ios := s.environment.nextStep.ios;
+// 
+//                 assert gls[k-1].ls == s;
+//                 assert gls[k].ls == s';
+//                 assert forall i :: i in s.servers <==> i in s'.servers;
+//                 assert packets' == packets + (set io | io in ios && io.LIoOpSend? :: io.s);
+// 
+//                 // Then I have id in s'.servers
+//                 // I also have s'.servers == s.servers[id := s'servers[id]]
+// 
+//                 // Now it's either NodeGrant(s, s', ios) or NodeAccept(s, s', ios)
+// 
+//                 if (NodeGrant(s.servers[id], s'.servers[id], ios)) {
+//                     if (s.servers[id].held && s.servers[id].epoch < 0xFFFF_FFFF_FFFF_FFFF) {
+//                         assert |ios| == 1;
+//                         assert ios[0].LIoOpSend?;
+//                         assert ios[0].s.msg.Transfer?;
+//                         assert forall p ::
+//                                       p in packets
+//                                    && p.src in s.servers
+//                                    && p.dst in s.servers
+//                                    && p.msg.Locked?
+//                                  <==> p in packets'
+//                                   && p.src in s'.servers
+//                                   && p.dst in s'.servers
+//                                   && p.msg.Locked?;
+//                     } else {
+//                     }
+//                 }
+// 
+//                 assert LS_GLS_Correspondence(ls[k].environment.sentPackets, gls[k]);
+//             } else {
+//                 assert false;
+//                 // Should be something like same valid locked messages in packets and packets'
+//             }
+//         }
+//         assert LS_GLS_Correspondence(ls[k].environment.sentPackets, gls[k]);
+//         k := k + 1;
+//     }
+// }
+
 
 
 lemma GLSToSS(config:Config, gls:seq<GLS_State>) returns (ss:seq<ServiceState>)
@@ -168,10 +257,68 @@ ensures forall i :: 0 <= i < |ss| ==> ss[i].history == gls[i].history
         assert(ss[i].history == gls[i].history);
         i := i + 1;
     }
-//    assert(ss[0].hosts == serverAddresses);
-//    assert(exists e :: e in serverAddresses && ss[0].history == [e]);
-//    assert(Service_Init(ss[0], serverAddresses));
 }
+
+
+// lemma sameHosts(ss:seq<ServiceState>) 
+// requires |ss| > 0
+// requires exists serverAddresses :: Service_Init(ss[0], serverAddresses)
+// requires forall i :: 0 <= i < |ss|-1 ==> Service_Next(ss[i], ss[i+1]) || ss[i] == ss[i+1]
+// ensures forall i :: 0 <= i < |ss| ==> ss[i].hosts == ss[0].hosts
+// {
+//     assert ss[0].hosts == ss[0].hosts;
+//     var k := 1;
+//     while (k < |ss|)
+//     invariant 1 <= k <= |ss|
+//     invariant forall i :: 0 <= i < k ==> ss[i].hosts == ss[0].hosts
+//     {
+//         assert forall i :: 0 <= i < |ss|-1 ==> Service_Next(ss[i], ss[i+1]) || ss[i] == ss[i+1];
+//         var kk := k-1;
+//         assert Service_Next(ss[kk], ss[kk+1]) || ss[kk] == ss[kk+1];
+//         assert ss[k] == ss[k-1] || Service_Next(ss[k-1], ss[k]);
+//         assert ss[k].hosts == ss[k-1].hosts;
+//         assert forall i :: 0 <= i <= k ==> ss[i].hosts == ss[0].hosts;
+//         k := k + 1;
+//     }
+// }
+
+
+
+lemma RefinementProof(config:Config, ls:seq<LS_State>) returns (ss:seq<ServiceState>)
+requires |ls| > 0
+requires LS_Init(ls[0], config)
+requires forall i :: 0 <= i < |ls|-1 ==> LS_Next(ls[i], ls[i+1]) || ls[i] == ls[i+1]
+ensures |ss| == |ls|
+ensures exists serverAddresses :: Service_Init(ss[0], serverAddresses)
+ensures forall i :: 0 <= i < |ss|-1 ==> Service_Next(ss[i], ss[i+1]) || ss[i] == ss[i+1]
+ensures forall i :: 0 <= i < |ls| ==> Protocol_Service_Correspondence(ls[i].environment.sentPackets, ss[i])
+{
+    var gls := LSToGLS(config, ls);
+    ss := GLSToSS(config, gls);
+
+    assert Protocol_Service_Correspondence(ls[0].environment.sentPackets, ss[0]);
+
+    var    k := 0;
+    while (k < |ls|-1)
+    invariant 0 <= k <= |ls|-1
+    invariant forall i :: 0 <= i <= k ==> Protocol_Service_Correspondence(ls[i].environment.sentPackets, ss[i])
+    {
+        assert forall i :: 0 <= i <= k ==> Protocol_Service_Correspondence(ls[i].environment.sentPackets, ss[i]);
+        if (ls[k] == ls[k+1]) {
+            // assert gls[k+1] == gls[k];
+            assert ss[k+1] == ss[k];
+            assert ls[k+1] == ls[k] ==> Protocol_Service_Correspondence(ls[k+1].environment.sentPackets, ss[k+1]);
+        } else {
+            assert LS_Next(ls[k], ls[k+1]);
+
+            assert Protocol_Service_Correspondence(ls[k+1].environment.sentPackets, ss[k+1]);
+        }
+        k := k + 1;
+    }
+}
+
+
+
 
 
 }
