ironfleet/src/Dafny/Distributed/LockProof/p_s_correspondence.s.dfy
@@ -1,0 +1,22 @@
+include "../Protocol/Lock/RefinementProof/DistributedSystem.i.dfy"
+include "../Protocol/Lock/Node.i.dfy"
+include "../Services/Lock/AbstractService.s.dfy"
+
+module P_S_Correspondence_s {
+import opened DistributedSystem_i
+import opened Protocol_Node_i
+import opened AbstractServiceLock_s
+
+predicate Protocol_Service_Correspondence(packets:set<LockPacket>, serviceState:ServiceState) {
+    
+    forall p :: 
+           p in packets
+        && p.src in serviceState.hosts
+        && p.dst in serviceState.hosts
+        && p.msg.Locked?
+        ==> var epoch := p.msg.locked_epoch;
+                0 < epoch <= |serviceState.history|
+            && p.src == serviceState.history[epoch-1]
+}
+
+}
