ironfleet/src/Dafny/Distributed/LockProof/p_s_lemma.i.dfy
@@ -1,0 +1,287 @@
+include "../Protocol/Lock/RefinementProof/DistributedSystem.i.dfy"
+include "../Protocol/Lock/Node.i.dfy"
+include "../Services/Lock/AbstractService.s.dfy"
+include "p_s_correspondence.s.dfy"
+
+
+module P_S_Lemma {
+import opened DistributedSystem_i
+import opened Protocol_Node_i
+import opened AbstractServiceLock_s
+import opened P_S_Correspondence_s
+
+lemma Incremental_Packets(ls:seq<LS_State>, config:Config)
+requires |ls| > 0
+requires LS_Init(ls[0], config)
+requires forall i :: 0 <= i < |ls|-1 ==> LS_Next(ls[i], ls[i+1]) || ls[i] == ls[i+1]
+ensures forall i :: 0 <= i < |ls|-1 ==> ls[i].environment.sentPackets <= ls[i+1].environment.sentPackets
+{
+}
+
+
+lemma sameConfig(config:Config, ls:seq<LS_State>)
+requires |ls| > 0
+requires LS_Init(ls[0], config)
+requires forall i :: 0 <= i < |ls|-1 ==> LS_Next(ls[i], ls[i+1]) || ls[i] == ls[i+1]
+ensures forall i :: 0 <= i < |ls| ==> forall j :: j in ls[i].servers ==> ls[i].servers[j].config == config
+{
+    assert forall j :: j in ls[0].servers ==> ls[0].servers[j].config == config;
+    
+    var k := 1;
+    while (k < |ls|) 
+    invariant 1 <= k <= |ls|
+    invariant forall i :: 0 <= i < k ==> forall j :: j in ls[i].servers ==> ls[i].servers[j].config == config;
+    {
+        assert forall i :: 0 <= i < k ==> forall j :: j in ls[i].servers ==> ls[i].servers[j].config == config;
+        assert 0 <= k-1 < |ls|-1;
+        assert (ls[k-1] == ls[k] || LS_Next(ls[k-1], ls[k]));
+        assert forall j :: j in ls[k].servers ==> ls[k].servers[j].config == ls[k-1].servers[j].config;
+        assert forall i :: 0 <= i <= k ==> forall j :: j in ls[i].servers ==> ls[i].servers[j].config == config;
+        k := k + 1;
+    }
+}
+
+lemma sameServers(config:Config, ls:seq<LS_State>)
+requires |ls| > 0
+requires LS_Init(ls[0], config)
+requires forall i :: 0 <= i < |ls|-1 ==> LS_Next(ls[i], ls[i+1]) || ls[i] == ls[i+1]
+ensures forall i :: 0 <= i < |ls| ==> (forall j :: j in config <==> j in ls[i].servers)
+{
+    assert forall j :: j in config <==> j in ls[0].servers;
+    var k := 1;
+    while (k < |ls|) 
+    invariant 1 <= k <= |ls|
+    invariant forall i :: 0 <= i < k ==> (forall j :: j in config <==> j in ls[i].servers)
+    {
+        var kk := k-1;
+        assert (ls[kk+1] == ls[kk] || LS_Next(ls[kk], ls[kk+1]));
+        assert forall j :: j in ls[k].servers <==> j in ls[k-1].servers;
+        assert forall j :: j in config <==> j in ls[k].servers;
+        k := k + 1;
+    }
+}
+
+
+predicate LS_GLS_Correspondence(packets:set<LockPacket>, gls:GLS_State, config:Config) {
+    
+    forall p ::
+           p in packets
+        && p.src in config
+        && p.dst in config
+        && p.msg.Locked?
+        ==> var epoch := p.msg.locked_epoch;
+                0 < epoch <= |gls.history|
+            && p.src == gls.history[epoch-1]
+}
+
+predicate LS_GLS_Transfer_Correspondence(packets:set<LockPacket>, gls:GLS_State, config:Config) {
+    
+    forall p ::
+           p in packets
+        && p.src in config
+        && p.dst in config
+        && p.msg.Transfer?
+        ==> var epoch := p.msg.transfer_epoch;
+                0 < epoch <= |gls.history|
+            && p.src == gls.history[epoch-1]
+}
+
+predicate Transfer_Epoch_In_History(gls:GLS_State, config:Config) {
+    forall p ::
+           p in gls.ls.environment.sentPackets
+        && p.msg.Transfer?
+        && p.src in config
+       ==> 2 <= p.msg.transfer_epoch <= |gls.history|
+}
+
+predicate Hold_Epoch(gls:GLS_State) {
+    forall s :: s in gls.ls.servers
+             && gls.ls.servers[s].held
+            ==> gls.ls.servers[s].epoch == |gls.history|
+}
+
+predicate Unique_Hold(s:LS_State) {
+    forall x, y :: 
+           x in s.servers 
+        && y in s.servers 
+        && s.servers[x].held 
+        && s.servers[y].held
+       ==> x == y 
+}
+
+lemma History_Len(gls:seq<GLS_State>, config:Config)
+requires |gls| > 0
+requires GLS_Init(gls[0], config)
+requires forall i :: 0 <= i < |gls|-1 ==> GLS_Next(gls[i], gls[i+1]) || gls[i] == gls[i+1]
+ensures forall i :: 0 <= i < |gls| ==> |gls[i].history| >= 1
+{}
+
+lemma At_Most_One_Hold(config:Config, ls:seq<LS_State>)
+requires |ls| > 0
+requires LS_Init(ls[0], config)
+requires forall i :: 0 <= i < |ls|-1 ==> LS_Next(ls[i], ls[i+1]) || ls[i] == ls[i+1]
+ensures forall i :: 0 <= i < |ls| ==> Unique_Hold(ls[i]);
+{
+    assert Unique_Hold(ls[0]);
+    var k := 1;
+    while (k < |ls|)
+    invariant 1 <= k <= |ls|
+    invariant forall i :: 0 <= i < k ==> Unique_Hold(ls[i])
+    {
+        var kk := k-1;
+
+        if (LS_Next(ls[kk], ls[kk+1])
+         && ls[kk].environment.nextStep.LEnvStepHostIos?
+         && ls[kk].environment.nextStep.actor in ls[kk].servers) {
+            var s := ls[kk];
+            var s' := ls[kk+1];
+            var id := s.environment.nextStep.actor;
+            var ios := s.environment.nextStep.ios;
+            assert s'.servers == s.servers[id := s'.servers[id]];
+            
+            forall x | x in s'.servers 
+            ensures !s'.servers[x].held
+            {
+                if (x != id) {
+                    assert s'.servers[x].held == s.servers[x] == false;
+                } else {
+                    assert !s'.servers[x].held;
+                }
+            }
+
+            assert Unique_Hold(ls[kk+1]);
+        } 
+        
+        k := k + 1;
+    }
+}
+
+lemma Hold_Epoch_Next(s:GLS_State, s':GLS_State)
+requires GLS_Next(s, s')
+requires s.ls.environment.nextStep.LEnvStepHostIos?
+requires s.ls.environment.nextStep.actor in s.ls.servers
+requires NodeGrant(s.ls.servers[s.ls.environment.nextStep.actor], s'.ls.servers[s.ls.environment.nextStep.actor], s.ls.environment.nextStep.ios)
+requires s.ls.servers[s.ls.environment.nextStep.actor].held
+requires s.ls.servers[s.ls.environment.nextStep.actor].epoch < 0xFFFF_FFFF_FFFF_FFFF
+requires Hold_Epoch(s)
+ensures Hold_Epoch(s')
+{
+    forall ss |
+           ss in s'.ls.servers
+        && s'.ls.servers[ss].held
+    ensures s'.ls.servers[ss].epoch == |s'.history|
+    {
+        var id := s.ls.environment.nextStep.actor;
+        if (ss == id) {
+            assert !s'.ls.servers[ss].held;
+        } else {
+            assert s'.ls.servers[ss] == s.ls.servers[ss];
+            assert s'.ls.servers[ss].epoch == |s.history|;
+        }
+    }
+
+}
+
+
+lemma Transfer_Epoch_In_History_Next(s:GLS_State, s':GLS_State, config:Config)
+requires GLS_Next(s, s')
+requires s.ls.environment.nextStep.LEnvStepHostIos?
+requires s.ls.environment.nextStep.actor in s.ls.servers
+requires NodeGrant(s.ls.servers[s.ls.environment.nextStep.actor], s'.ls.servers[s.ls.environment.nextStep.actor], s.ls.environment.nextStep.ios)
+requires s.ls.servers[s.ls.environment.nextStep.actor].held
+requires s.ls.servers[s.ls.environment.nextStep.actor].epoch < 0xFFFF_FFFF_FFFF_FFFF
+requires forall j :: j in s.ls.servers ==> s.ls.servers[j].config == config
+requires forall j :: j in config <==> j in s.ls.servers
+requires Transfer_Epoch_In_History(s, config)
+requires s.ls.environment.nextStep.ios[0].s.msg.transfer_epoch == |s'.history|;
+requires |s'.history| > 1
+ensures Transfer_Epoch_In_History(s', config)
+{
+    var ios := s.ls.environment.nextStep.ios;
+    var id := s.ls.environment.nextStep.actor;
+    assert |ios| == 1;
+    assert ios[0].s.msg.Transfer?;
+    // sameServers(config, ls);
+    // sameConfig(config, ls);
+    //assert LS_Next(s.ls, s'.ls);
+    //assert LEnvironment_Next(s.ls.environment, s'.ls.environment);
+    assert IsValidLIoOp(s.ls.environment.nextStep.ios[0], s.ls.environment.nextStep.actor, s.ls.environment);
+    assert ios[0].s.src == id;
+    assert ios[0].s.src in config;
+    forall p |
+           p in s'.ls.environment.sentPackets
+        && p.msg.Transfer?
+        && p.src in config
+    ensures 2 <= p.msg.transfer_epoch <= |s'.history|
+    {
+        if (p == ios[0].s) {
+            assert p.msg.transfer_epoch == |s'.history|;
+            assert 2 <= p.msg.transfer_epoch <= |s'.history|;
+        }
+    }
+}
+
+
+lemma Receive_Next(s:GLS_State, s':GLS_State, config:Config)
+requires GLS_Next(s, s')
+requires s.ls.environment.nextStep.LEnvStepHostIos?
+requires s.ls.environment.nextStep.actor in s.ls.servers
+requires s.ls.environment.nextStep.LEnvStepHostIos?
+requires s.ls.environment.nextStep.actor in s.ls.servers
+requires NodeAccept(s.ls.servers[s.ls.environment.nextStep.actor], s'.ls.servers[s.ls.environment.nextStep.actor], s.ls.environment.nextStep.ios)
+requires s.ls.environment.nextStep.ios[0].LIoOpReceive?
+requires !s.ls.servers[s.ls.environment.nextStep.actor].held
+requires s.ls.environment.nextStep.ios[0].r.src in s.ls.servers[s.ls.environment.nextStep.actor].config
+requires s.ls.environment.nextStep.ios[0].r.msg.Transfer?
+requires s.ls.environment.nextStep.ios[0].r.msg.transfer_epoch > s.ls.servers[s.ls.environment.nextStep.actor].epoch
+requires s.ls.environment.sentPackets <= s'.ls.environment.sentPackets;
+requires forall j :: j in s.ls.servers ==> s.ls.servers[j].config == config
+requires forall j :: j in s'.ls.servers ==> s'.ls.servers[j].config == config
+requires Transfer_Epoch_In_History(s, config);
+requires LS_GLS_Correspondence(s.ls.environment.sentPackets, s, config)
+requires Hold_Epoch(s)
+ensures LS_GLS_Correspondence(s'.ls.environment.sentPackets, s', config)
+ensures Hold_Epoch(s')
+ensures Transfer_Epoch_In_History(s', config)
+{
+    var id := s.ls.environment.nextStep.actor;
+    var ios := s.ls.environment.nextStep.ios;
+    assert |ios| == 2;
+    assert ios[1].LIoOpSend?;
+
+    assert Transfer_Epoch_In_History(s',config);
+
+    assert ios[0].r in s.ls.environment.sentPackets;
+    assert ios[0].r.msg.Transfer?;
+    assert ios[0].r.src in s.ls.servers[id].config;
+
+    assert exists p ::
+                  p in s.ls.environment.sentPackets
+               && p.msg.Transfer?
+               && p.src in config
+               && p.msg.transfer_epoch == ios[1].s.msg.locked_epoch;
+    
+
+
+    assert 2 <= ios[1].s.msg.locked_epoch <= |s'.history|; 
+    assert s'.history[ios[1].s.msg.locked_epoch-1] == ios[1].s.src; //(3)
+
+
+
+    assert LS_GLS_Correspondence(s.ls.environment.sentPackets, s', config);
+    assert forall p ::
+           p in (set io | io in ios && io.LIoOpSend? :: io.s)
+        && p.src in config
+        && p.dst in config
+        && p.msg.Locked?
+        ==> 0 < p.msg.locked_epoch <= |s'.history|
+         && p.src == s'.history[p.msg.locked_epoch-1];
+    
+    assert LS_GLS_Correspondence(s'.ls.environment.sentPackets, s', config);
+    assert Hold_Epoch(s'); 
+
+
+}
+
+
+}
