ironfleet/src/Dafny/Distributed/LockProof/proof_re.i.dfy
@@ -1,0 +1,137 @@
+include "../Protocol/Lock/RefinementProof/DistributedSystem.i.dfy"
+include "../Protocol/Lock/Node.i.dfy"
+include "../Services/Lock/AbstractService.s.dfy"
+include "p_s_correspondence.s.dfy"
+include "p_s_lemma.i.dfy"
+
+
+module LockProof {
+import opened DistributedSystem_i
+import opened Protocol_Node_i
+import opened AbstractServiceLock_s
+import opened P_S_Correspondence_s
+import opened P_S_Lemma
+
+lemma LSToGLS(config:Config, ls:seq<LS_State>) returns (gls:seq<GLS_State>)
+requires |ls| > 0
+requires LS_Init(ls[0], config)
+requires forall i :: 0 <= i < |ls|-1 ==> LS_Next(ls[i], ls[i+1]) || ls[i] == ls[i+1]
+ensures |ls| == |gls|
+ensures GLS_Init(gls[0], config)
+ensures forall i :: 0 <= i < |gls|-1 ==> GLS_Next(gls[i], gls[i+1]) || gls[i] == gls[i+1]
+ensures forall i :: 0 <= i < |ls| ==> LS_GLS_Correspondence(ls[i].environment.sentPackets, gls[i], config)
+{
+    var k := 1;
+    gls := [GLS_State(ls[0], [config[0]])];
+    assert forall j :: j in ls[0].servers && ls[0].servers[j].held ==> ls[0].servers[j].epoch == |gls[0].history| && gls[0].history[|gls[0].history|-1] == j;
+
+    while (k < |ls|)
+    invariant 1 <= k <= |ls|
+    invariant |gls| == k
+    invariant GLS_Init(gls[0], config)
+    invariant forall i :: 0 <= i < k-1 ==> GLS_Next(gls[i], gls[i+1]) || gls[i] == gls[i+1]
+    invariant forall i :: 0 <= i < k ==> ls[i] == gls[i].ls
+    invariant forall i :: 0 <= i < k ==> LS_GLS_Correspondence(ls[i].environment.sentPackets, gls[i], config)
+    invariant forall i :: 0 <= i < k ==> Transfer_Epoch_In_History(gls[i], config)
+    invariant forall i :: 0 <= i < k ==> Hold_Epoch(gls[i])
+    //invariant forall i :: 0 <= i < k ==> LS_GLS_Transfer_Correspondence(ls[i].environment.sentPackets, gls[i], config)
+    // invariant forall i :: 0 <= i < k ==> forall j :: j in ls[i].servers && ls[i].servers[j].held ==> ls[i].servers[j].epoch == |gls[i].history| && gls[i].history[|gls[i].history|-1] == j
+    {
+
+        var kk := k-1;
+        var s  := ls[kk];
+        var s' := ls[kk+1];
+        var history := gls[kk].history;
+        var packets := s.environment.sentPackets;
+        var packets':= s'.environment.sentPackets;
+
+        if (LS_Next(s, s')) {
+
+            if (s.environment.nextStep.LEnvStepHostIos?) {
+
+                var id := s.environment.nextStep.actor;
+                var ios:= s.environment.nextStep.ios;
+
+                if (s.environment.nextStep.actor in s.servers) {
+
+                    if (NodeGrant(s.servers[id], s'.servers[id], ios)) {
+
+                        if (s.servers[id].held && s.servers[id].epoch < 0xFFFF_FFFF_FFFF_FFFF) {
+
+                            history := history + [s.servers[id].config[(s.servers[id].my_index + 1) % |s.servers[id].config|]];
+                            gls := gls + [GLS_State(s', history)];
+                            assert GLS_Next(gls[kk], gls[kk+1]);
+                            assert gls[kk+1].ls == s';
+
+                            assert s'.environment.sentPackets == s.environment.sentPackets + (set io | io in ios && io.LIoOpSend? :: io.s);
+                            assert LS_GLS_Correspondence(s'.environment.sentPackets, gls[kk+1], config);
+                            assert ios[0].s.msg.transfer_epoch == |gls[kk+1].history|;
+                            sameServers(config, ls);
+                            sameConfig(config, ls);
+                            Transfer_Epoch_In_History_Next(gls[kk], gls[kk+1], config);
+                            assert Transfer_Epoch_In_History(gls[kk+1], config);
+                            assert Hold_Epoch(gls[kk]);
+                            Hold_Epoch_Next(gls[kk], gls[kk+1]);
+                            assert Hold_Epoch(gls[kk+1]);
+                        } else {
+
+                            gls := gls + [GLS_State(s', history)];
+                            assert GLS_Next(gls[kk], gls[kk+1]);
+                            assert LS_GLS_Correspondence(s'.environment.sentPackets, gls[kk+1], config);
+                        }
+
+
+                    } else { // NodeAccept(s.servers[id], s'.servers[id], ios)
+
+                        gls := gls + [GLS_State(s', history)];
+                        assert NodeAccept(s.servers[id], s'.servers[id], ios);
+                        assert |ios| >= 1;
+
+                        if (ios[0].LIoOpReceive?) {
+                        
+                            if (   !s.servers[id].held
+                                && ios[0].r.src in s.servers[id].config
+                                && ios[0].r.msg.Transfer?
+                                && ios[0].r.msg.transfer_epoch > s.servers[id].epoch) {
+
+                                    Incremental_Packets(ls, config);
+                                    sameConfig(config, ls);
+                                    Receive_Next(gls[kk], gls[kk+1], config);
+                                } else {
+                                
+                                    assert LS_GLS_Correspondence(s'.environment.sentPackets, gls[kk+1], config);
+                                    assert Transfer_Epoch_In_History(gls[kk+1], config);
+                                    assert Hold_Epoch(gls[kk+1]); 
+                                }
+                                assert Transfer_Epoch_In_History(gls[kk+1], config);
+                        } else {
+
+                            assert LS_GLS_Correspondence(s'.environment.sentPackets, gls[kk+1], config);
+                        }
+                        
+                        assert LS_GLS_Correspondence(s'.environment.sentPackets, gls[kk+1], config);
+                    }
+
+                } else { // ???
+
+                    gls := gls + [GLS_State(s', history)];
+                    sameServers(config, ls);
+                    assert LS_GLS_Correspondence(s'.environment.sentPackets, gls[kk+1], config);
+                    assert GLS_Next(gls[kk], gls[kk+1]);
+                }
+
+            } else { // s.environment.sentPackets == s'.environment.sentPackets
+                gls := gls + [GLS_State(s', history)];
+            }
+            
+        } else { // s == s'
+            
+            gls := gls + [GLS_State(s', history)];
+        }
+
+        k := k + 1;
+    }
+}
+
+
+}
